Draft redux of ExecA

src/reordering/ReorderingExecA.v
@@ -21,17 +21,11 @@ Section ExecA.
 
 Variable X_t X_t' X_s : WCore.t.
 Variable a_t b_t : actid.
+Variable l_a : label.
 
 Notation "'G_t'" := (WCore.G X_t).
 Notation "'G_t''" := (WCore.G X_t').
 Notation "'G_s'" := (WCore.G X_s).
-
-Notation "'R' G" := (fun e => is_true (is_r (lab G) e)) (at level 1).
-Notation "'F' G" := (fun e => is_true (is_f (lab G) e)) (at level 1).
-Notation "'W' G" := (fun e => is_true (is_w (lab G) e)) (at level 1).
-Notation "'Acq' G" := (fun e => is_true (is_acq (lab G) e)) (at level 1).
-Notation "'Rlx' G" := (fun e => is_true (is_rlx (lab G) e)) (at level 1).
-Notation "'Rel' G" := (fun e => is_true (is_rel (lab G) e)) (at level 1).
 
 Notation "'lab_t'" := (lab G_t).
 Notation "'val_t'" := (val lab_t).
@@ -61,8 +55,7 @@ Notation "'rf_t''" := (rf G_t').
 Notation "'co_t''" := (co G_t').
 Notation "'rmw_t''" := (rmw G_t').
 Notation "'rpo_t''" := (rpo G_t').
-Notation "'rhb_t''" := (rhb G_t').
-Notation "'hb_t''" := (hb G_t').
+Notation "'sw_t''" := (sw G_t').
 Notation "'rmw_dep_t''" := (rmw_dep G_t').
 Notation "'data_t''" := (data G_t').
 Notation "'ctrl_t''" := (ctrl G_t').
@@ -82,33 +75,401 @@ Notation "'rf_s'" := (rf G_s).
 Notation "'co_s'" := (co G_s).
 Notation "'rmw_s'" := (rmw G_s).
 Notation "'rpo_s'" := (rpo G_s).
+Notation "'sw_s'" := (sw G_s).
 Notation "'rmw_dep_s'" := (rmw_dep G_s).
 Notation "'data_s'" := (data G_s).
 Notation "'ctrl_s'" := (ctrl G_s).
 Notation "'addr_s'" := (addr G_s).
 Notation "'W_s'" := (fun x => is_true (is_w lab_s x)).
 Notation "'R_s'" := (fun x => is_true (is_r lab_s x)).
-Notation "'F_s'" := (F G_s).
+Notation "'F_s'" := (fun x => is_true (is_f G_s x)).
 Notation "'vf_s'" := (vf G_s).
 Notation "'srf_s'" := (srf G_s).
 Notation "'Loc_s_' l" := (fun e => loc_s e = l) (at level 1).
 Notation "'Val_s_' l" := (fun e => val_s e = l) (at level 1).
-Notation "'Rlx_s'" := (Rlx G_s).
-Notation "'Acq_s'" := (Acq G_s).
-Notation "'Rel_s'" := (Rel G_s).
+Notation "'Rlx_s'" := (fun x => is_true (is_rlx G_s x)).
+Notation "'Acq_s'" := (fun x => is_true (is_acq G_s x)).
+Notation "'Rel_s'" := (fun x => is_true (is_rel G_s x)).
 
+Notation "'is_init'" := (fun e => is_true (is_init e)).
 Notation "'Tid_' t" := (fun e => tid e = t) (at level 1).
 Notation "'mapper'" := (mapper a_t b_t).
 
+Notation "'A_s'" := (extra_a X_t a_t b_t b_t).
+Notation "'B_s'" := (extra_a X_t a_t b_t a_t).
+Notation "'A_s''" := (extra_a X_t' a_t b_t b_t).
+
+Definition rsr_a_Gs_prime := {|
+  acts_set := E_s;
+  threads_set := threads_set G_s;
+  lab := upd lab_s b_t l_a;
+  rf := rf_s ⨾ ⦗E_s \₁ eq b_t⦘ ∪
+        mapper ↑ (rf_t' ⨾ ⦗eq a_t⦘);
+  co := restr_rel (E_s \₁ eq b_t) co_s ∪
+        mapper ↑ (⦗eq a_t⦘ ⨾ co_t' ∪ co_t' ⨾ ⦗eq a_t⦘);
+  rmw := mapper ↑ rmw_t';
+  rmw_dep := rmw_dep_s;
+  ctrl := ctrl_s;
+  data := data_s;
+  addr := addr_s;
+|}.
+
+Definition rsr_a_Xs_prime := {|
+  WCore.G := rsr_a_Gs_prime;
+  WCore.sc := WCore.sc X_s;
+|}.
+
+Notation "'X_s''" := rsr_a_Xs_prime.
+Notation "'G_s''" := (WCore.G X_s').
+Notation "'lab_s''" := (lab G_s').
+Notation "'val_s''" := (val lab_s').
+Notation "'loc_s''" := (loc lab_s').
+Notation "'same_loc_s''" := (same_loc lab_s').
+Notation "'E_s''" := (acts_set G_s').
+Notation "'loc_s''" := (loc lab_s').
+Notation "'sb_s''" := (sb G_s').
+Notation "'rf_s''" := (rf G_s').
+Notation "'co_s''" := (co G_s').
+Notation "'rmw_s''" := (rmw G_s').
+Notation "'rpo_s''" := (rpo G_s').
+Notation "'sw_s''" := (sw G_s').
+Notation "'rmw_dep_s''" := (rmw_dep G_s').
+Notation "'data_s''" := (data G_s').
+Notation "'ctrl_s''" := (ctrl G_s').
+Notation "'addr_s''" := (addr G_s').
+Notation "'W_s''" := (fun x => is_true (is_w lab_s' x)).
+Notation "'R_s''" := (fun x => is_true (is_r lab_s' x)).
+Notation "'F_s''" := (fun x => is_true (is_f lab_s' x)).
+Notation "'vf_s''" := (vf G_s').
+Notation "'srf_s''" := (srf G_s').
+Notation "'Loc_s_'' l" := (fun e => loc_s' e = l) (at level 1).
+Notation "'Val_s_'' l" := (fun e => val_s' e = l) (at level 1).
+Notation "'Rlx_s''" := (fun e => is_true (is_rlx lab_s' e)).
+Notation "'Acq_s''" := (fun e => is_true (is_acq lab_s' e)).
+Notation "'Rel_s''" := (fun e => is_true (is_rel lab_s' e)).
+
+Hypothesis ADD : WCore.add_event X_t X_t' a_t l_a.
+
+Lemma rsr_step_acts : E_t' ≡₁ E_t ∪₁ eq a_t.
+Proof using ADD.
+  destruct ADD as (r & R1 & w & W1 & W2 & ADD').
+  apply ADD'.
+Qed.
+
+Lemma rsr_at_tid : tid a_t <> tid_init.
+Proof using ADD.
+  destruct ADD as (r & R1 & w & W1 & W2 & ADD').
+  apply ADD'.
+Qed.
+
+Lemma rsr_at_ninit : ~is_init a_t.
+Proof using ADD.
+  destruct ADD as (r & R1 & w & W1 & W2 & ADD').
+  apply ADD'.
+Qed.
+
+Lemma rsr_at_notin : ~E_t a_t.
+Proof using ADD.
+  destruct ADD as (r & R1 & w & W1 & W2 & ADD').
+  apply ADD'.
+Qed.
+
+Lemma rsr_at_in' : E_t' a_t.
+Proof using ADD.
+  apply rsr_step_acts. now right.
+Qed.
+
+Lemma rsr_step_lab : lab_t' = upd lab_t a_t l_a.
+Proof using ADD.
+  destruct ADD as (r & R1 & w & W1 & W2 & ADD').
+  apply ADD'.
+Qed.
+
+Hint Resolve rsr_at_tid rsr_at_notin rsr_at_ninit
+             rsr_at_in' : xmm.
+
 Hypothesis INV : reord_step_pred X_t a_t b_t.
 Hypothesis INV' : reord_step_pred X_t' a_t b_t.
+Hypothesis CONS : WCore.is_cons G_t'.
 
-Lemma prefix_exec_restr_eq X X' d
-    (SUB : d ⊆₁ acts_set (WCore.G X))
-    (PFX : SubToFullExec.prefix X X') :
-  WCore.exec_restr_eq X X' d.
+Lemma rsr_bt_in' : E_t' b_t.
+Proof using ADD INV'.
+  apply (rsr_at_bt_ord INV'), rsr_at_in'.
+Qed.
+
+Lemma rsr_bt_in : E_t b_t.
+Proof using ADD INV'.
+  clear - ADD INV'.
+  assert (NEQ : a_t <> b_t) by apply INV'.
+  assert (IN' : E_t' b_t) by apply rsr_bt_in'.
+  apply rsr_step_acts in IN'.
+  unfolder in IN'. desf.
+Qed.
+
+Lemma rsr_old_exa : A_s ≡₁ eq b_t.
+Proof using ADD INV'.
+  apply extra_a_some; auto with xmm.
+  apply rsr_bt_in.
+Qed.
+
+Lemma rsr_new_exa : A_s' ≡₁ ∅.
+Proof using ADD INV'.
+  apply extra_a_none_l; auto with xmm.
+Qed.
+
+Hint Resolve rsr_bt_in' rsr_bt_in : xmm.
+
+Hypothesis SIMREL : reord_simrel X_s X_t a_t b_t mapper.
+
+Lemma rsr_nanb_lab : eq_dom E_t' lab_t' (lab_s' ∘ mapper).
+Proof using ADD SIMREL INV INV'.
+  assert (NEQ : a_t <> b_t) by apply INV.
+  simpl.
+  rewrite <- rsr_mapper_at with (a_t := a_t) (b_t := b_t) at 1.
+  all: auto.
+  rewrite rsr_step_lab, <- upd_compose; auto with xmm.
+  rewrite rsr_step_acts. apply eq_dom_union. split.
+  { apply eq_dom_upd; auto with xmm.
+    symmetry. apply SIMREL. }
+  apply eq_dom_eq. now rewrite !upds.
+Qed.
+
+Lemma rsr_nanb_lab' : eq_dom E_t' (lab_s' ∘ mapper) lab_t'.
+Proof using ADD SIMREL INV INV'.
+  symmetry. exact rsr_nanb_lab.
+Qed.
+
+Lemma rsr_nanb_mapinj : inj_dom E_t' mapper.
+Proof using ADD SIMREL INV INV'.
+  assert (NEQ : a_t <> b_t) by apply INV.
+  eapply inj_dom_mori; auto with xmm.
+  red; auto with hahn.
+Qed.
+
+Hint Resolve rsr_nanb_lab rsr_nanb_lab'
+            rsr_nanb_mapinj rsr_Gt_wf : xmm.
+
+Definition f := @id actid.
+Definition cmt := E_s \₁ eq b_t.
+Definition dtrmt := E_s \₁ (eq b_t ∪₁ eq a_t).
+Definition thrdle :=
+  eq tid_init × set_compl (eq tid_init) ∪
+  set_compl (eq (tid b_t)) × eq (tid b_t).
+
+Lemma rsr_a_labeq : eq_dom dtrmt lab_s' lab_s.
 Proof using.
+  simpl.
+  apply eq_dom_upd_l; [| reflexivity].
+  unfold dtrmt. clear. unfolder. tauto.
+Qed.
+
+Lemma rsr_a_sb_same : sb_s' ≡ sb_s.
+Proof using ADD SIMREL INV INV'.
+  unfold sb at 1. simpl.
+  now change (⦗E_s⦘ ⨾ ext_sb ⨾ ⦗E_s⦘) with sb_s.
+Qed.
+
+Lemma rsr_a_sb_helper :
+  dom_rel (sb_t ⨾ ⦗eq b_t⦘) × eq a_t ≡
+    WCore.sb_delta a_t (E_t \₁ eq b_t).
+Proof using ADD SIMREL INV INV'.
+  assert (BNINI : ~is_init b_t) by apply INV.
+  assert (BTID : tid b_t <> tid_init) by apply (rsr_bt_tid INV).
+  unfold WCore.sb_delta. apply cross_more; [| reflexivity].
+  rewrite sb_tid_init', unionC.
+  rewrite !seq_union_l, seqA, dom_union.
+  arewrite (same_tid a_t ≡₁ same_tid b_t).
+  { unfold same_tid. now rewrite (rsr_at_bt_tid INV). }
+  split.
+  { apply set_union_mori; [basic_solver |].
+    rewrite <- seq_eqv_inter_lr.
+    arewrite (sb_t ⨾ ⦗eq b_t⦘ ⊆ ⦗E_t \₁ eq b_t⦘ ⨾ sb_t ⨾ ⦗eq b_t⦘)
+      ; [| basic_solver].
+    rewrite wf_sbE at 1. rewrite !seqA.
+    unfolder. ins. desf. splits; auto.
+    intro FALSO. desf. eapply sb_irr; eauto. }
+  apply set_union_mori.
+  { unfold sb, ext_sb. unfolder.
+    ins. desf. eexists; splits.
+    all: desf; eauto with xmm.
+    now apply (rsr_init_acts INV). }
+  intros x XIN.
+  destruct sb_total
+      with (G := G_t) (t := tid b_t)
+           (a := b_t) (b := x)
+        as [SB|SB].
+  { unfolder; splits; auto with xmm. }
+  { assert (TEQ : tid b_t = tid x) by apply XIN.
+    unfolder; splits; auto; try apply XIN.
+    unfold is_init; desf. }
+  { apply XIN. }
+  { exfalso. apply (rsr_bt_max INV) with b_t x.
+    all: auto with xmm.
+    assert (BIN : E_t b_t) by auto with xmm.
+    basic_solver. }
+  exists b_t.
+  enough (same_tid b_t x) by basic_solver.
+  apply XIN.
+Qed.
+
+Lemma rsr_a_sb :
+  sb_s' ≡ mapper ↑ swap_rel sb_t' (eq b_t ∩₁ E_t') (eq a_t ∩₁ E_t').
+Proof using ADD SIMREL INV INV'.
+  assert (NEQ : a_t <> b_t) by apply INV.
+  assert (BNINI : ~is_init b_t) by apply INV.
+  assert (ANIN : ~E_t a_t) by auto with xmm.
+  assert (STID : same_tid a_t b_t) by apply INV.
+  destruct ADD as (r & R1 & w & W1 & W2 & ADD').
+  rewrite (WCore.add_event_sb ADD'), swap_rel_unionE.
+  rewrite rsr_a_sb_same, (rsr_sb SIMREL).
+  arewrite (eq a_t ∩₁ E_t ≡₁ ∅).
+  { split; auto with hahn.
+    unfolder. intros x (XEQ & XIN). subst x.
+    auto with xmm. }
+  rewrite !set_inter_absorb_r, swap_rel_empty_r.
+  all: try (red; ins; subst x; auto with xmm).
+  rewrite rsr_old_exa; auto.
+  rewrite <- rsr_mapper_at
+     with (a_t := a_t) (b_t := b_t)
+       at 4 5; auto.
+  rewrite <- !set_collect_eq, <- !collect_rel_cross,
+          <- !collect_rel_union.
+  apply collect_rel_more; auto.
+  unfold swap_rel.
+  arewrite (
+    WCore.sb_delta a_t E_t \ eq b_t × eq a_t ≡
+      WCore.sb_delta a_t (E_t \₁ eq b_t)
+  ).
+  { unfold WCore.sb_delta. rewrite <- cross_minus_l.
+    apply cross_more; [| reflexivity].
+    rewrite set_minus_union_l.
+    apply set_union_more; [| basic_solver].
+    rewrite set_minus_disjoint; basic_solver. }
+  arewrite (sb_t \ eq b_t × eq a_t ≡ sb_t).
+  { rewrite minus_disjoint; [reflexivity |].
+    rewrite wf_sbE. basic_solver. }
+  rewrite <- rsr_a_sb_helper. basic_solver 11.
+Qed.
+
+Lemma rsr_oldacts : mapper ↑₁ E_t ⊆₁ E_s \₁ eq b_t.
+Proof using ADD SIMREL INV INV'.
+  now rewrite (rsr_codom SIMREL), rsr_old_exa.
+Qed.
+
+Lemma rsr_a_rf : rf_s' ≡ mapper ↑ rf_t'.
+Proof using ADD SIMREL INV INV'.
+  assert (WF_t : Wf G_t) by apply INV.
+  destruct ADD as (r & R1 & w & W1 & W2 & ADD').
+  simpl.
+  rewrite (rsr_rf SIMREL), (rf_delta_RE WF_t ADD'),
+          !seq_union_l.
+  arewrite_false ((srf_s ⨾ ⦗A_s ∩₁ R_s⦘) ⨾ ⦗E_s \₁ eq b_t⦘).
+  { rewrite rsr_old_exa. basic_solver. }
+  rewrite (WCore.add_event_rf ADD'),
+          (add_event_to_rf_complete ADD' WF_t (rsr_Gt_rfc INV)).
+  rewrite !union_false_r, collect_rel_union.
+  apply union_more; [| reflexivity].
+  split; [basic_solver 11 |].
+  rewrite (wf_rfE WF_t) at 1.
+  rewrite !collect_rel_seqi, !collect_rel_eqv,
+          rsr_oldacts.
+  basic_solver 11.
+Qed.
+
+Lemma rsr_a_co : co_s' ≡ mapper ↑ co_t'.
+Proof using ADD SIMREL INV INV'.
+  assert (WF_t : Wf G_t) by apply INV.
+  destruct ADD as (r & R1 & w & W1 & W2 & ADD').
+  simpl.
+  rewrite (rsr_co SIMREL), (co_deltaE WF_t ADD'),
+          restr_union.
+  arewrite_false (
+    restr_rel
+      (E_s \₁ eq b_t)
+      (add_max
+        (extra_co_D E_s lab_s (loc_s b_t))
+        (A_s ∩₁ W_s))
+  ).
+  { rewrite rsr_old_exa. basic_solver. }
+  rewrite (WCore.add_event_co ADD').
+  rewrite union_false_r, collect_rel_union.
+  apply union_more; [| reflexivity].
+  split; [basic_solver 11 |].
+  rewrite (wf_coE WF_t) at 1.
+  rewrite !collect_rel_seqi, !collect_rel_eqv,
+          rsr_oldacts.
+  basic_solver 11.
+Qed.
+
+Lemma rsr_a_acts : E_s' ≡₁ mapper ↑₁ E_t'.
+Proof using ADD SIMREL INV INV'.
+  assert (NEQ : a_t <> b_t) by apply (rsr_at_neq_bt INV).
+  destruct ADD as (r & R1 & w & W1 & W2 & ADD').
+  simpl.
+  rewrite (rsr_acts SIMREL), (WCore.add_event_acts ADD'),
+          set_collect_union, set_collect_eq, rsr_old_exa.
+  rewrite rsr_mapper_at; auto with hahn.
+Qed.
+
+Hint Resolve rsr_a_labeq : xmm.
+
+Lemma rsr_a_sim :
+  reord_simrel X_s' X_t' a_t b_t mapper.
+Proof using ADD SIMREL INV INV'.
+  destruct ADD as (r & R1 & w & W1 & W2 & ADD').
+  assert (ANINI : ~is_init a_t) by apply INV.
+  assert (BNINI : ~is_init b_t) by apply INV.
+  assert (WF_t : Wf G_t) by apply INV.
+  assert (NEQ : a_t <> b_t) by apply (rsr_at_neq_bt INV).
+  assert (TEQ : tid a_t = tid b_t) by apply (rsr_at_bt_tid INV).
   constructor.
+  all: rewrite ?rsr_new_exa.
+  all: rewrite ?set_minus_empty_r, ?set_union_empty_r,
+               ?set_inter_empty_l, ?cross_false_l, ?cross_false_r,
+               ?eqv_empty,
+               ?seq_false_r, ?add_max_empty_r, ?union_false_r.
+  all: auto with xmm hahn.
+  { apply rsr_a_acts. }
+  { eapply eq_dom_mori; eauto with xmm.
+    red. auto with hahn. }
+  { apply rsr_a_acts. }
+  { apply rsr_a_sb. }
+  { apply rsr_a_rf. }
+  { apply rsr_a_co. }
+  { now rewrite (WCore.add_event_threads ADD'), <- (rsr_threads SIMREL). }
+  all: simpl.
+  all: rewrite ?(WCore.add_event_ctrl ADD'), ?(WCore.add_event_data ADD'),
+               ?(WCore.add_event_addr ADD'), ?(WCore.add_event_rmw_dep ADD').
+  all: try now apply SIMREL.
+  { rewrite rsr_step_acts, !set_minus_minus_l.
+    arewrite ((E_t ∪₁ eq a_t) \₁ (eq a_t ∪₁ eq b_t) ≡₁ E_t \₁ eq b_t).
+    { rewrite set_minus_union_l, set_unionC.
+      rewrite !set_minus_union_r, set_minusK.
+      rewrite set_minus_disjoint
+         with (s1 := E_t) (s2 := eq a_t)
+            ; [basic_solver |].
+      unfolder. intros x XIN XEQ. subst x. auto with xmm. }
+    intros x XIN. rewrite rsr_mappero.
+    all: forward apply XIN; unfold id.
+    all: try (clear; basic_solver).
+    unfolder. ins. desf. intro FALSO. subst x.
+    auto with xmm. }
+  all: rewrite set_inter_absorb_r.
+  all: try (red; ins; subst x; auto with xmm).
+  all: rewrite set_collect_eq, ?rsr_mapper_bt,
+               ?rsr_mapper_at.
+  all: auto with hahn.
+Qed.
+
+Lemma rsr_a_pfx :
+  SubToFullExec.prefix (WCore.X_start X_s dtrmt) X_s'.
+Proof using ADD SIMREL INV INV'.
+Admitted.
+
+Lemma rsr_a_restr_eq :
+  WCore.exec_restr_eq (WCore.X_start X_s dtrmt) X_s cmt.
+Proof using ADD SIMREL INV INV'.
+  (* constructor.
   all: try now apply PFX.
   { rewrite !set_inter_absorb_l; ins.
     now rewrite <- (prf_acts PFX). }
@@ -120,586 +481,38 @@ Proof using.
   { now rewrite (prf_rmw PFX), restr_restr, set_inter_absorb_l. }
   { now rewrite (prf_data PFX). }
   { now rewrite (prf_ctrl PFX). }
-  now rewrite (prf_rmw_dep PFX).
-Qed.
+  now rewrite (prf_rmw_dep PFX). *)
+Admitted.
 
-Lemma simrel_exec_a l
-    (NSC : WCore.sc X_s ≡ ∅₂)
-    (SIMREL : reord_simrel X_s X_t a_t b_t mapper)
-    (STEP : WCore.exec_inst X_t X_t' a_t l) :
-  exists X_s' f' dtrmt' cmt',
-    << SIMREL : reord_simrel X_s' X_t' a_t b_t mapper >> /\
-    << STEP : WCore.reexec X_s X_s' f' dtrmt' cmt' >>.
-Proof using INV INV'.
-  assert (CORR : reord_step_pred X_t a_t b_t); ins.
-  assert (CORR' : reord_step_pred X_t' a_t b_t); ins.
-  (* Setup vars *)
-  destruct STEP as [ADD RFC CONS].
-  destruct ADD as (r & R1 & w & W1 & W2 & ADD).
-  set (G_s' := {|
-    acts_set := E_s;
-    threads_set := threads_set G_s;
-    lab := upd lab_s b_t l;
-    rf := rf_s ⨾ ⦗E_s \₁ eq b_t⦘ ∪
-          mapper ↑ (rf_t' ⨾ ⦗eq a_t⦘);
-    co := restr_rel (E_s \₁ eq b_t) co_s ∪
-          mapper ↑ (⦗eq a_t⦘ ⨾ co_t') ∪
-          mapper ↑ (co_t' ⨾ ⦗eq a_t⦘);
-    rmw := mapper ↑ rmw_t';
-    rmw_dep := rmw_dep_s;
-    ctrl := ctrl_s;
-    data := data_s;
-    addr := addr_s;
-  |}).
-  set (X_s' := {|
-    WCore.sc := WCore.sc X_s;
-    WCore.G := G_s';
-  |}).
-  set (cmt' := E_s \₁ eq b_t).
-  set (dtrmt' := E_s \₁ eq b_t \₁ eq (mapper b_t)).
-  set (thrdle' :=
-    eq tid_init × set_compl (eq tid_init) ∪
-    set_compl (eq (tid b_t)) × eq (tid b_t)
-  ).
-  assert (NEQ : a_t <> b_t) by apply CORR.
-  assert (TEQ : tid a_t = tid b_t) by apply CORR.
-  assert (INB' : E_t' b_t).
-  { apply (rsr_at_bt_ord CORR'), (WCore.add_event_acts ADD).
-    now right. }
-  assert (INB : E_t b_t).
-  { apply (WCore.add_event_acts ADD) in INB'.
-    destruct INB' as [INB' | EQ]; ins. }
-  assert (WF : Wf G_t) by apply CORR.
-  assert (WF' : Wf G_t').
-  { apply CORR'. }
-  assert (ENINIT : ~is_init a_t) by apply ADD.
-  assert (NOTINA : ~E_t a_t).
-  { apply ADD. }
-  assert (INA : E_t' a_t) by (apply ADD; now right).
-  assert (AINS : E_s b_t).
-  { apply (rsr_acts SIMREL). unfold extra_a. desf.
-    { basic_solver. }
-    exfalso; eauto. }
-  assert (BINS : E_s (mapper b_t)).
-  { rewrite rsr_mapper_bt; auto.
-    apply (rsr_acts SIMREL). left.
-    exists b_t. split; eauto with xmm. }
-  assert (NOEXA : extra_a X_t' a_t b_t b_t ≡₁ ∅).
-  { unfold extra_a; desf. desf. }
-  assert (OLDEXA : extra_a X_t a_t b_t b_t ≡₁ eq b_t).
-  { unfold extra_a; desf. exfalso; eauto. }
-  assert (MAPER_E : mapper ↑₁ eq a_t ≡₁ eq b_t).
-  { rewrite set_collect_eq. apply set_equiv_single_single.
-    eauto with xmm. }
-  assert (ANCODOM : ~ (mapper ↑₁ E_t) b_t).
-  { intro FALSO. apply (rsr_codom SIMREL) in FALSO.
-    now apply FALSO, OLDEXA. }
-  assert (MAPNEQ : forall x (IN : E_t x), mapper x <> b_t).
-  { intros x XIN EQ. apply (rsr_codom SIMREL) with (x := b_t).
-    { basic_solver. }
-    now apply OLDEXA. }
-  assert (NEWSBSIM : sb G_s' ≡ mapper ↑ swap_rel sb_t' (eq b_t ∩₁ E_t') (eq a_t ∩₁ E_t')).
-  { change (sb G_s') with sb_s.
-    rewrite (rsr_sb SIMREL), OLDEXA.
-    arewrite (eq a_t ∩₁ E_t ≡₁ ∅) by basic_solver.
-    arewrite (eq b_t ∩₁ E_t' ≡₁ eq b_t) by basic_solver.
-    arewrite (eq a_t ∩₁ E_t' ≡₁ eq a_t).
-    { rewrite (WCore.add_event_acts ADD). basic_solver. }
-    rewrite swap_rel_empty_r, (WCore.add_event_sb ADD),
-            swap_rel_union.
-    unfold swap_rel. rewrite !collect_rel_union.
-    arewrite (sb_t \ eq b_t × eq a_t ≡ sb_t).
-    { rewrite minus_disjoint; ins. unfold sb.
-      rewrite <- restr_relE, restr_relEE.
-      basic_solver. }
-    unfold WCore.sb_delta. rewrite <- cross_minus_l.
-    rewrite !collect_rel_cross, MAPER_E.
-    arewrite (mapper ↑₁ eq b_t ≡₁ eq (mapper b_t)).
-    { rewrite set_collect_eq. unfold mapper. rupd; ins. }
-    arewrite ((is_init ∪₁ E_t ∩₁ same_tid a_t) \₁ eq b_t ≡₁
-              dom_rel (sb_t ⨾ ⦗eq b_t⦘)).
-    { rewrite sb_tid_init', seq_union_l, unionC, dom_union,
-              set_minus_union_l.
-      assert (NINIT : ~is_init b_t) by apply INV.
-      arewrite (is_init \₁ eq b_t ≡₁ is_init).
-      { split; [basic_solver|]. unfolder.
-        ins. split; ins. intro FALSO; congruence. }
-      arewrite (same_tid a_t ≡₁ same_tid b_t).
-      { unfold same_tid. now rewrite (rsr_at_bt_tid INV). }
-      apply set_union_more.
-      { unfold sb. split; [|basic_solver 11].
-        unfolder. ins. eexists. splits; eauto.
-        { apply (rsr_init_acts INV); ins. }
-        unfold ext_sb. desf; ins. }
-      rewrite wf_sbE, <- seq_eqv_inter_lr, !seqA, <- id_inter.
-      rewrite set_inter_absorb_l
-          with (s := eq b_t)
-            by basic_solver.
-      unfolder. unfold same_tid.
-      split; intros x HREL; desf; splits; ins.
-      all: try now (intro FALSO; desf; eapply sb_irr; eauto).
-      eexists; splits; eauto.
-      destruct (sb_total G_t)
-          with (tid b_t) x b_t
-            as [RSB|LSB].
-      all: ins; try congruence.
-      { unfolder; splits; ins. intro FALSO; destruct x; ins.
-        apply (rsr_at_tid CORR). now rewrite (rsr_at_bt_tid CORR). }
-      exfalso. apply (rsr_bt_max CORR) with b_t x; ins.
-      basic_solver 11. }
-    basic_solver 12. }
-  assert (SIMREL' : reord_simrel X_s' X_t' a_t b_t mapper).
-  { constructor; ins.
-    { eapply inj_dom_mori; eauto with xmm.
-      red; auto with hahn. }
-    { rewrite NOEXA. basic_solver. }
-    { rewrite (WCore.add_event_acts ADD), set_collect_union,
-              (rsr_codom SIMREL), NOEXA, OLDEXA.
-      rewrite set_collect_eq, rsr_mapper_at; auto.
-      basic_solver. }
-    { apply SIMREL. }
-    { eapply eq_dom_mori; eauto with xmm.
-      red. auto with hahn. }
-    { rewrite (WCore.add_event_acts ADD), (WCore.add_event_lab ADD).
-      apply eq_dom_union; split; ins.
-      { unfolder. intros x XIN.
-        rewrite <- rsr_mapper_at
-           with (a_t := a_t) (b_t := b_t)
-             at 1; auto.
-        rewrite <- upd_compose; auto with xmm.
-        rewrite !updo by congruence.
-        apply (rsr_lab SIMREL); ins. }
-      unfolder. ins. desf. unfold compose.
-      rewrite rsr_mapper_at; auto. now rupd. }
-    { rewrite (WCore.add_event_acts ADD), NOEXA,
-              set_union_empty_r, set_collect_union,
-              (rsr_acts SIMREL).
-      now rewrite OLDEXA, set_collect_eq, rsr_mapper_at. }
-    { now rewrite NOEXA, cross_false_l, cross_false_r,
-              !union_false_r. }
-    { rewrite NOEXA, set_inter_empty_l,
-              (rsr_rf SIMREL), seq_union_l, OLDEXA.
-      rewrite (rf_delta_RE (rsr_Gt_wf CORR) ADD).
-      arewrite_false ((srf_s ⨾ ⦗eq b_t ∩₁ R_s⦘) ⨾ ⦗E_s \₁ eq b_t⦘).
-      { clear. basic_solver. }
-      rewrite eqv_empty, seq_false_r, !union_false_r,
-              (WCore.add_event_rf ADD), !collect_rel_union.
-      arewrite (mapper ↑ rf_t ⨾ ⦗E_s \₁ eq b_t⦘ ≡ mapper ↑ rf_t).
-      { split; [clear; basic_solver 7|].
-        rewrite (wf_rfE WF), <- OLDEXA, <- (rsr_codom SIMREL).
-        clear. basic_solver. }
-      rewrite (add_event_to_rf_complete ADD).
-      all: try now apply CORR.
-      now rewrite collect_rel_empty, !union_false_r. }
-    { rewrite NOEXA, set_inter_empty_l, add_max_empty_r,
-              union_false_r.
-      rewrite (co_deltaE1 WF ADD),
-              (co_deltaE2 WF ADD).
-      rewrite (WCore.add_event_co ADD). unfold WCore.co_delta.
-      rewrite !collect_rel_union, <- !unionA.
-      repeat apply union_more; ins.
-      rewrite (rsr_co SIMREL), restr_union.
-      arewrite (restr_rel (E_s \₁ eq b_t) (mapper ↑ co_t) ≡ mapper ↑ co_t).
-      { split; [clear; basic_solver 11 |].
-        rewrite <- OLDEXA, <- (rsr_codom SIMREL),
-                collect_rel_restr, restr_relE.
-        { apply collect_rel_mori; ins. apply WF. }
-        eapply inj_dom_mori with (x := E_t); eauto; [| apply SIMREL].
-        unfold flip. rewrite (wf_coE WF). clear. basic_solver. }
-      rewrite restr_add_max, OLDEXA.
-      arewrite (eq b_t ∩₁ W_s ∩₁ (E_s \₁ eq b_t) ≡₁ ∅).
-      { clear. basic_solver. }
-      rewrite add_max_empty_r, union_false_r.
-      apply collect_rel_eq_dom' with (s := E_t); ins.
-      apply (wf_coE (rsr_Gt_wf CORR)). }
-    { now rewrite (rsr_threads SIMREL), (WCore.add_event_threads ADD). }
-    { rewrite (WCore.add_event_ctrl ADD). apply SIMREL. }
-    { rewrite (WCore.add_event_data ADD). apply SIMREL. }
-    { rewrite (WCore.add_event_addr ADD). apply SIMREL. }
-    { rewrite (WCore.add_event_rmw_dep ADD). apply SIMREL. }
-    { unfolder. ins. desf.
-      unfold id. auto with xmm. }
-    { unfolder. ins. desf.
-      rewrite rsr_mapper_bt; auto. }
-    unfolder. ins. desf.
-    rewrite rsr_mapper_at; auto. }
-  assert (PFX : SubToFullExec.prefix (WCore.X_start X_s dtrmt') X_s').
-  { assert (DT : dtrmt' ∩₁ E_s ≡₁ dtrmt').
-    { unfold dtrmt'. basic_solver. }
-    assert (INIT : is_init ⊆₁ dtrmt').
-    { unfold dtrmt'.
-      rewrite <- sico_init_acts_s; [| | apply INV].
-      all: try now (eapply rsr_common; eauto).
-      unfolder. intros x XNIT.
-      splits; ins.
-      all: intro FALSO; subst x.
-      { eapply rsr_as_ninit with (X_t := X_t); eauto.
-        now apply OLDEXA. }
-      assert (TID : (tid ∘ mapper) b_t = tid_init).
-      { unfold compose. destruct (mapper b_t); ins. }
-      rewrite (rsr_tid SIMREL) in TID; ins.
-      apply (rsr_at_tid INV).
-      now rewrite (rsr_at_bt_tid INV). }
-    unfold X_s'. constructor; ins.
-    { now rewrite DT, INIT. }
-    { basic_solver. }
-    { rewrite DT, INIT, set_unionK.
-      unfold dtrmt'. unfolder; ins; desf.
-      rupd. congruence. }
-    { unfolder. ins. rupd. congruence. }
-    { rewrite DT, restr_union, restr_relE,
-              !seqA, <- id_inter.
-      arewrite ((E_s \₁ eq b_t) ∩₁ dtrmt' ≡₁ dtrmt').
-      { unfold dtrmt'. basic_solver. }
-      arewrite_false (restr_rel dtrmt' (mapper ↑ (rf_t' ⨾ ⦗eq a_t⦘)));
-        [| clear; basic_solver].
-      rewrite collect_rel_seqi, collect_rel_eqv,
-              set_collect_eq, restr_relE, !seqA.
-      rewrite rsr_mapper_at; auto.
-      unfold dtrmt'. clear. basic_solver. }
-    { rewrite DT, !restr_union, !restr_relE,
-              !seqA, <- !id_inter.
-      seq_rewrite <- !id_inter.
-      rewrite set_interC.
-      arewrite ((E_s \₁ eq b_t) ∩₁ dtrmt' ≡₁ dtrmt').
-      { unfold dtrmt'. clear. basic_solver. }
-      arewrite_false (⦗dtrmt'⦘ ⨾ mapper ↑ (⦗eq a_t⦘ ⨾ co_t')).
-      { rewrite collect_rel_seqi, collect_rel_eqv,
-                set_collect_eq, rsr_mapper_at; auto.
-        unfold dtrmt'. clear. basic_solver. }
-      arewrite_false (mapper ↑ (co_t' ⨾ ⦗eq a_t⦘) ⨾ ⦗dtrmt'⦘).
-      { rewrite collect_rel_seqi, collect_rel_eqv,
-                set_collect_eq, rsr_mapper_at; auto.
-        unfold dtrmt'. clear. basic_solver. }
-      now rewrite seq_false_l, seq_false_r, !union_false_r. }
-    { rewrite DT, (WCore.add_event_rmw ADD),
-              collect_rel_union, restr_union,
-              !restr_relE, (rsr_rmw SIMREL).
-      arewrite_false (mapper ↑ WCore.rmw_delta a_t r ⨾ ⦗dtrmt'⦘).
-      { unfold WCore.rmw_delta.
-        rewrite collect_rel_cross, set_collect_eq, rsr_mapper_at; auto.
-        unfold dtrmt'. clear. basic_solver. }
-      now rewrite seq_false_r, union_false_r. }
-    { rewrite (rsr_data SIMREL), (rsr_ndata CORR). basic_solver. }
-    { rewrite (rsr_ctrl SIMREL), (rsr_nctrl CORR). basic_solver. }
-    { rewrite (rsr_addr SIMREL), (rsr_naddr CORR). basic_solver. }
-    { rewrite (rsr_rmw_dep SIMREL), (rsr_nrmw_dep CORR). basic_solver. }
-    { rewrite NSC. clear. basic_solver. }
-    unfold SubExecution.restrict. rewrite wf_sbE; ins.
-    unfold sb at 2. ins.
-    rewrite !seqA, <- id_inter, set_interC, !DT.
-    unfolder. intros x y (XINE & SB & YD).
-    splits; ins; [| red in SB; unfolder in SB; desf].
-    apply (rsr_sb SIMREL') in SB.
-    destruct SB as [[SB | ESB] | ESB].
-    { destruct SB as (x' & y' & SB & XEQ & YEQ).
-      subst. unfold swap_rel in SB.
-      assert (YNB : y' <> b_t).
-      { intro FALSO. apply YD. subst y'.
-        unfold mapper. rupd. congruence. }
-      assert (YNA : y' <> a_t).
-      { intro FALSO. destruct YD as [YD _].
-        apply YD. subst y'.
-        unfold mapper. now rupd. }
-      destruct SB as [SB | EX]; [|unfolder in EX; desf].
-      destruct SB as [SB BAN].
-      assert (XNA : x' <> a_t).
-      { intro FALSO; subst. apply (WCore.add_event_sb ADD) in SB.
-        destruct SB as [SB|SB].
-        all: unfold sb in SB; unfolder in SB.
-        all: desf. }
-      assert (XNB : x' <> b_t).
-      { intro FALSO; subst. apply (WCore.add_event_sb ADD) in SB.
-        destruct SB as [SB|SB].
-        all: unfold sb in SB; unfolder in SB.
-        all: desf.
-        eapply (rsr_bt_max INV); ins.
-        unfold sb; basic_solver. }
-      assert (XIN : E_t x').
-      { unfold sb in SB. unfolder in SB.
-        destruct SB as (SB & _ & _).
-        apply (WCore.add_event_acts ADD) in SB.
-        destruct SB; congruence. }
-      unfold dtrmt'.
-      rewrite rsr_mapper_bt, rsr_mappero; auto.
-      rewrite rsr_mappero in XINE; auto.
-      unfold dtrmt'. unfolder; splits; auto. }
-    { enough (YIN : extra_a X_t' a_t b_t b_t y).
-      { exfalso. apply extra_a_none_l in YIN; auto. }
-      apply ESB. }
-    enough (XIN : extra_a X_t' a_t b_t b_t x).
-    { exfalso. apply extra_a_none_l in XIN; auto. }
-    apply ESB. }
-  assert (STARTWF : WCore.wf (WCore.X_start X_s dtrmt') X_s' cmt').
-  { constructor; ins.
-    { apply prefix_wf with (X := WCore.X_start X_s dtrmt') (X' := X_s').
-      all: ins.
-      { rewrite (rsr_data SIMREL), (rsr_ndata INV). basic_solver. }
-      { rewrite (rsr_addr SIMREL), (rsr_naddr INV). basic_solver. }
-      { rewrite (rsr_ctrl SIMREL), (rsr_nctrl INV). basic_solver. }
-      { rewrite (rsr_rmw_dep SIMREL), (rsr_nrmw_dep INV). basic_solver. }
-      eapply G_s_wf with (X_s := X_s') (X_t := X_t'); eauto. }
-    { apply prefix_exec_restr_eq; ins.
-      basic_solver. }
-    { unfold rf_complete, G_s', cmt'. ins.
-      arewrite ((E_s \₁ eq b_t) ∩₁ E_s ≡₁ E_s \₁ eq b_t).
-      { basic_solver. }
-      arewrite ((E_s \₁ eq b_t) ∩₁ is_r (upd lab_s b_t l) ≡₁
-                (E_s \₁ eq b_t) ∩₁ R_s).
-      { unfolder. split; ins; desf; splits; ins.
-        all: unfold is_r in *.
-        all: rewrite updo in *; congruence. }
-      rewrite seq_union_l, seq_union_r, !seqA.
-      rewrite codom_union.
-      arewrite_false (mapper ↑ (rf_t' ⨾ ⦗eq a_t⦘) ⨾ ⦗E_s \₁ eq b_t⦘).
-      { rewrite collect_rel_seqi, collect_rel_eqv,
-                set_collect_eq, rsr_mapper_at; auto.
-        clear. basic_solver. }
-      rewrite seq_false_r, codom_empty, set_union_empty_r.
-      seq_rewrite seq_eqvK. unfolder.
-      intros x ((XINE & NEQ') & ISR).
-      assert (RFC_S : rf_complete G_s).
-      { eapply G_s_rfc with (X_t := X_t); eauto. }
-      assert (WF_S : Wf G_s).
-      { eapply G_s_wf with (X_t := X_t); eauto. }
-      destruct RFC_S with x
-            as (xw & RF); [split; ins|].
-      exists xw; splits; ins.
-      { apply (wf_rfE WF_S) in RF.
-        unfolder in RF; desf. }
-      intro FALSO; subst xw.
-      apply (rsr_rf SIMREL) in RF.
-      destruct RF as [RFT | SRF].
-      { unfolder in RFT.
-        destruct RFT as (x' & y' & RFT & EQ & _).
-        apply MAPNEQ with x'; ins.
-        apply (wf_rfE WF) in RFT.
-        unfolder in RFT; desf. }
-      unfolder in SRF. destruct SRF as (_ & EXA & _).
-      apply OLDEXA in EXA. congruence. }
-    unfold dtrmt', cmt'. basic_solver 11. }
-  assert (STAB : WCore.stable_uncmt_reads_gen X_s' cmt' thrdle').
-  { constructor; ins.
-    { unfold thrdle'. clear. basic_solver. }
-    { unfold thrdle'. clear - INV.
-      unfolder. ins. desf.
-      now apply (rsr_bt_tid INV). }
-    { constructor; unfold thrdle'.
-      { clear. basic_solver. }
-      clear - INV. unfolder. ins. desf.
-      { exfalso. now apply (rsr_bt_tid INV). }
-      left. split; auto.
-      intro FALSO.
-      now apply (rsr_bt_tid INV). }
-    arewrite (E_s \₁ cmt' ≡₁ eq b_t).
-    { subst cmt'. rewrite !set_minus_minus_r.
-      basic_solver. }
-    arewrite (
-      vf G_s' ⨾ same_tid ⊆
-        (vf G_s' ⨾ same_tid) \ same_tid ∪
-        (vf G_s' ⨾ same_tid) ∩ same_tid
-    ).
-    { rewrite unionC.
-      rewrite <- split_rel
-         with (s := ⊤₁) (s' := ⊤₁).
-      reflexivity. }
-    rewrite seq_union_l.
-    apply union_mori; [| basic_solver].
-    unfolder. unfold thrdle', same_tid.
-    clear. basic_solver. }
-  assert (CONS' : WCore.is_cons G_s').
-  { change G_s' with (WCore.G X_s').
-    eapply rsr_cons with (X_t := X_t'); eauto. }
-  assert (DINC : dtrmt' ⊆₁ cmt').
-  { subst dtrmt' cmt'. basic_solver. }
-  (* The proof *)
-  exists X_s', id, dtrmt', cmt'.
-  split; red; ins.
-  red. exists thrdle'.
-  constructor; ins.
-  { assert (BNINI : ~is_init b_t) by apply INV.
-    unfold dtrmt'. rewrite <- (rsr_init_acts_s INV SIMREL).
-    rewrite rsr_mapper_bt; auto.
-    clear - ENINIT BNINI.
-    unfolder. ins. desf. splits; congruence. }
-  { subst cmt'. basic_solver. }
-  { rewrite (rsr_sbE INV SIMREL).
-    rewrite extra_a_some; auto.
-    rewrite !seq_union_l, !seq_union_r.
-    rewrite <- cross_inter_r.
-    arewrite (eq a_t ∩₁ dtrmt' ≡₁ ∅).
-    { unfold dtrmt'. rewrite rsr_mapper_bt; auto.
-      clear. basic_solver. }
-    rewrite !cross_false_r, seq_false_r, !union_false_r.
-    unfold dtrmt'.
-    rewrite (rsr_actsE INV SIMREL), extra_a_some; auto.
-    rewrite rsr_mapper_bt; auto.
-    clear - INB NOTINA INV. unfolder.
-    intros x y (SB & (YIN & YEQ) & YNEQ).
-    splits; auto.
-    { red in SB; unfolder in SB; desf. eauto. }
-    { intro FALSO. subst x.
-      apply (rsr_bt_max INV) with b_t y; auto.
-      basic_solver. }
-    intro FALSO. subst x.
-    red in SB; unfolder in SB; desf. }
-  { enough (SUB :
-      ⦗dtrmt'⦘ ⨾ immediate (nin_sb G_s') ⨾ ⦗cmt' \₁ dtrmt'⦘ ⊆ ∅₂
-    ).
-    { rewrite (set_union_minus DINC).
-      rewrite id_union, !seq_union_r.
-      apply inclusion_union_l; auto with hahn.
-      rewrite SUB. clear. basic_solver. }
-    change G_s' with (WCore.G X_s').
-    rewrite (rsr_sbE_imm INV' SIMREL'), (extra_sbE INV' SIMREL').
-    rewrite NOEXA, cross_false_l, union_false_r.
-    arewrite (cmt' \₁ dtrmt' ≡₁ eq a_t).
-    { unfold cmt', dtrmt'. rewrite rsr_mapper_bt; auto.
-      rewrite !set_minus_minus_r.
-      rewrite (rsr_actsE INV SIMREL), extra_a_some; auto.
-      clear - NOTINA INB NEQ. split; [| basic_solver 11].
-      arewrite (((E_t ∪₁ eq a_t) \₁ eq b_t) ∩₁ eq a_t ≡₁ eq a_t).
-      { basic_solver. }
-      arewrite (((E_t ∪₁ eq a_t) \₁ eq b_t) ∩₁ eq b_t ≡₁ ∅).
-      { basic_solver. }
-      rewrite set_minus_minus_l, set_minus_union_r,
-              set_minusK, set_inter_empty_r.
-      now rewrite !set_union_empty_l. }
-    arewrite (
-      immediate (nin_sb G_t') ⨾ ⦗eq a_t⦘ ⊆
-        ⦗eq b_t⦘ ⨾ immediate (nin_sb G_t') ⨾ ⦗eq a_t⦘
-    ).
-    { clear - INV' INA INB'. red. intros x y IMM.
-      exists x. split; auto. unfolder. split; auto.
-      red in IMM. destruct IMM as (y' & IMM & (EQ & EQ')).
-      subst y' y.
-      eapply nin_sb_functional_l; eauto; [apply INV' |].
-      apply seq_eqv_imm. exists b_t. split.
-      { unfolder. split; auto. apply INV'. }
-      eapply (rsr_at_bt_imm INV'). basic_solver. }
-    unfold dtrmt'. clear. basic_solver. }
+Lemma rsr_a_cfg_wf :
+  WCore.wf (WCore.X_start X_s dtrmt) X_s' cmt.
+Proof using ADD SIMREL INV INV'.
+Admitted.
+
+Lemma rsr_a_surg :
+  WCore.stable_uncmt_reads_gen X_s' cmt thrdle.
+Proof using ADD SIMREL INV INV'.
+Admitted.
+
+Lemma rsr_a_step :
+  WCore.reexec X_s X_s' f dtrmt cmt.
+Proof using.
+  red. exists thrdle. constructor.
   { admit. }
-  { constructor; ins.
-    { unfold id; ins. rupd. intro FALSO.
-      now apply CMT. }
-    { rewrite collect_rel_id. unfold rpo.
-      arewrite (restr_rel cmt' (rpo_imm G_s')⁺ ⊆ (restr_rel cmt' (rpo_imm G_s'))⁺).
-      { apply restr_rel_ct, rpo_imm_upward_closed.
-        unfold cmt'. admit. }
-      apply clos_trans_mori. unfold rpo_imm.
-      rewrite !restr_union, !restr_relE, !seqA.
-      arewrite (⦗cmt'⦘ ⨾ ⦗R G_s' ∩₁ Rlx G_s'⦘ ≡ ⦗R_s ∩₁ Rlx_s⦘ ⨾ ⦗cmt'⦘).
-      { unfold cmt'. unfolder.
-        split; ins; desf; splits; ins.
-        all: unfold is_r, is_rlx, mod in *.
-        all: rewrite updo in *; ins.
-        all: congruence. }
-      arewrite (⦗cmt'⦘ ⨾ ⦗Acq G_s'⦘ ≡ ⦗Acq_s⦘ ⨾ ⦗cmt'⦘).
-      { unfold cmt'. unfolder.
-        split; ins; desf; splits; ins.
-        all: unfold is_acq, mod in *.
-        all: rewrite updo in *; ins.
-        all: congruence. }
-      arewrite (⦗cmt'⦘ ⨾ ⦗F G_s' ∩₁ Rel G_s'⦘ ≡ ⦗F_s ∩₁ Rel_s⦘ ⨾ ⦗cmt'⦘).
-      { unfold cmt'. unfolder.
-        split; ins; desf; splits; ins.
-        all: unfold is_f, is_rel, mod in *.
-        all: rewrite updo in *; ins.
-        all: congruence. }
-      arewrite (⦗F G_s' ∩₁ Acq G_s'⦘ ⨾ ⦗cmt'⦘ ≡ ⦗cmt'⦘ ⨾ ⦗F_s ∩₁ Acq_s⦘).
-      { unfold cmt'. unfolder.
-        split; ins; desf; splits; ins.
-        all: unfold is_f, is_acq, mod in *.
-        all: rewrite updo in *; ins.
-        all: congruence. }
-      arewrite (⦗Rel G_s'⦘ ⨾ ⦗cmt'⦘ ≡ ⦗cmt'⦘ ⨾ ⦗Rel_s⦘).
-      { unfold cmt'. unfolder.
-        split; ins; desf; splits; ins.
-        all: unfold is_rel, mod in *.
-        all: rewrite updo in *; ins.
-        all: congruence. }
-      arewrite (⦗W G_s' ∩₁ Rlx G_s'⦘ ⨾ ⦗cmt'⦘ ≡ ⦗cmt'⦘ ⨾ ⦗W_s ∩₁ Rlx_s⦘).
-      { unfold cmt'. unfolder.
-        split; ins; desf; splits; ins.
-        all: unfold is_w, is_rlx, mod in *.
-        all: rewrite updo in *; ins.
-        all: congruence. }
-      seq_rewrite <- !restr_relE.
-      now arewrite (restr_rel cmt' (sb G_s') ⊆ sb_s). }
-    { rewrite collect_rel_id, restr_union.
-      apply inclusion_union_l; [basic_solver |].
-      unfolder. intros x y ((x' & y' & (RF & EQ) & XEQ & YEQ) & CX & CY).
-      exfalso. apply CY. rewrite <- YEQ, <- EQ.
-      symmetry. auto with xmm. }
-    { rewrite collect_rel_id, !restr_union.
-      repeat apply inclusion_union_l; [basic_solver | |].
-      { unfolder. intros x y ((x' & y' & (EQ & CO) & XEQ & YEQ) & CX & CY).
-        exfalso. apply CX. rewrite <- XEQ, <- EQ.
-        symmetry. auto with xmm. }
-      unfolder. intros x y ((x' & y' & (CO & EQ) & XEQ & YEQ) & CX & CY).
-      exfalso. apply CY. rewrite <- YEQ, <- EQ.
-      symmetry. auto with xmm. }
-    { rewrite collect_rel_id, (WCore.add_event_rmw ADD), collect_rel_union,
-              restr_union.
-      rewrite (rsr_rmw SIMREL).
-      apply inclusion_union_l; [clear; basic_solver 11 |].
-      unfolder. intros x y ((x' & y' & (RO & EQ) & XEQ & YEQ) & CX & CY).
-      exfalso. apply CY. rewrite <- YEQ, <- EQ.
-      symmetry. auto with xmm. }
-    arewrite (id ↑₁ cmt' ≡₁ cmt').
-    { clear. basic_solver. }
-    unfold cmt'. clear. basic_solver. }
-  { apply (G_s_rfc INV' SIMREL'). }
-  { arewrite (WCore.reexec_thread X_s' dtrmt' ≡₁ eq (tid b_t)).
-    { unfold dtrmt', WCore.reexec_thread. ins.
-      rewrite rsr_mapper_bt, !set_minus_minus_r; auto.
-      rewrite set_minusK, set_inter_absorb_l; [| basic_solver].
-      rewrite set_union_empty_l, set_collect_union, set_union_absorb_r.
-      { clear. basic_solver. }
-      clear - TEQ. basic_solver. }
-    unfold dtrmt'. rewrite (rsr_acts SIMREL), OLDEXA.
-    rewrite rsr_mapper_bt; auto.
-    clear - TEQ NEQ INB NOTINA. rewrite !set_minus_union_l.
-    rewrite !set_minus_minus_l. split; [| basic_solver].
-    unfolder.
-    intros x' [(x & (XIN & XEQ)) | XEQ]; [| desf; eauto].
-    subst x'.
-    assert (XNA : x <> a_t) by congruence.
-    destruct classic with (x = b_t) as [XEQ | XNB].
-    { subst x. right. split; eauto.
-      erewrite <- rsr_mapper_tid; eauto.
-      all: done. }
-    do 2 left. split; eauto. rewrite rsr_mappero; auto.
-    apply and_not_or; split; congruence. }
-  apply sub_to_full_exec_listless with (thrdle := thrdle'); ins.
-  { eapply G_s_rfc with (X_s := X_s'); eauto. }
-  { arewrite (E_s \₁ dtrmt' ∩₁ E_s ≡₁ eq b_t ∪₁ eq (mapper b_t)).
-    { rewrite set_minus_inter_r, set_minusK, set_union_empty_r.
-      subst dtrmt'.
-      rewrite !set_minus_minus_r, set_minusK, set_union_empty_l.
-      rewrite !set_inter_absorb_l; ins; [| basic_solver].
-      rewrite (rsr_acts SIMREL). basic_solver. }
-    apply set_finite_union. split; apply set_finite_eq. }
-  { eapply G_s_wf with (X_s := X_s'); eauto. }
-  { unfold dtrmt'.
-    rewrite set_inter_absorb_r; [| basic_solver].
-    rewrite !set_minus_minus_r, set_minusK, set_union_empty_l.
-    apply set_subset_union_l. split.
-    { unfolder. intros x (INE & XEQ) FALSO. subst x.
-      eapply rsr_as_ninit with (x := b_t) (X_t := X_t); eauto.
-      { apply extra_a_some; ins. }
-      eapply rsr_ninit_acts_s with (X_t := X_t); eauto.
-      red; eauto. }
-    unfolder. intros x (INE & XEQ) FALSO. subst x.
-    assert (INIT : is_init b_t).
-    { change (tid (mapper b_t)) with ((tid ∘ mapper) b_t) in FALSO.
-      rewrite (rsr_tid SIMREL) in FALSO; ins.
-      apply (rsr_ninit_acts CORR). split; ins. }
-    apply (rsr_bt_ninit CORR); ins. }
-  { now rewrite (rsr_data SIMREL), (rsr_ndata CORR). }
-  { now rewrite (rsr_addr SIMREL), (rsr_naddr CORR). }
-  { now rewrite (rsr_ctrl SIMREL), (rsr_nctrl CORR). }
-  now rewrite (rsr_rmw_dep SIMREL), (rsr_nrmw_dep CORR).
+  { admit. }
+  { admit. }
+  { admit. }
+  { apply rsr_a_surg. }
+  { admit. }
+  { admit. }
+  { admit. }
+  { admit. }
+  { apply (G_s_rfc INV' rsr_a_sim). }
+  { apply rsr_a_cfg_wf. }
+  { eapply rsr_cons with (X_t := X_t'); eauto.
+    apply rsr_a_sim. }
+  { admit. }
+  admit.
 Admitted.
 
 End ExecA.
